equivalent_as_node_list_entails_both_lengths_are_equal 를 알아서 증명 못 하다니? 정말 '길이'에 대해서는 어렵구나.

src/study/Nemonuri.Study.CSharpSyntaxRewriter2.Modifier2/Nemonuri.StratifiedNodes.Nodes.Equivalence.fst
@@ -5,14 +5,14 @@ module I = Nemonuri.StratifiedNodes.Internals
 module N = Nemonuri.StratifiedNodes.Nodes.Base
 open Nemonuri.StratifiedNodes.Nodes.Bijections
 
-//--- theory members ---
+//--- private theory members ---
 
-let are_equivalent_as_node #t #node_level 
+private let are_equivalent_as_node_impl #t #node_level 
   (node:N.node t) (node_internal:I.node_internal t node_level)
   : Tot bool =
   (to_node node_internal = node)
 
-let are_equivalent_as_node_list #t #node_list_level
+private let are_equivalent_as_node_list_impl #t #node_list_level
   (node_list:N.node_list t) (node_list_internal:I.node_list_internal t node_list_level)
   : Pure bool True
     (ensures fun b -> 
@@ -33,28 +33,91 @@ let are_equivalent_as_node_list_entails_get_item_pair_are_equivalent_as_node
   (node_list_internal:I.node_list_internal t node_list_level)
   (index:nat)
   : prop =
-  ((are_equivalent_as_node_list node_list node_list_internal) /\
+  ((are_equivalent_as_node_list_impl node_list node_list_internal) /\
   (index < (L.length node_list))) ==>
-  (are_equivalent_as_node 
+  (are_equivalent_as_node_impl 
     (L.index node_list index) (I.get_item node_list_internal index))
+
+let equivalent_as_node_list_entails_any_item_pair_are_equivalent_as_node
+  (t: eqtype)
+  : prop =
+  forall (node_list_level:nat) (node_list:N.node_list t)
+  (node_list_internal:I.node_list_internal t node_list_level) (index:nat).
+  (are_equivalent_as_node_list_entails_get_item_pair_are_equivalent_as_node
+    node_list node_list_internal index)
+
+let equivalent_as_node_list_entails_both_lengths_are_equal
+  (t: eqtype)
+  : prop =
+  forall (node_list_level:nat) (node_list:N.node_list t)
+  (node_list_internal:I.node_list_internal t node_list_level).
+  (L.length node_list) = (I.get_length node_list_internal)
+
+let equivalent_theorem (t:eqtype) : prop =
+  equivalent_as_node_list_entails_any_item_pair_are_equivalent_as_node t
 
 //---|
 
 //--- lemma ---
 
-(*
-let lemma_are_equivalent_as_node_list_entails_get_item_pair_are_equivalent_as_node
+let rec lemma_are_equivalent_as_node_list_entails_get_item_pair_are_equivalent_as_node
   #t #node_list_level
   (node_list:N.node_list t) 
   (node_list_internal:I.node_list_internal t node_list_level)
   (index:nat)
   : Lemma 
-    (requires (are_equivalent_as_node_list node_list node_list_internal) /\
-      (index < (L.length node_list)))
-    (ensures (are_equivalent_as_node 
-      (L.index node_list index) (I.get_item node_list_internal index)))
+    (ensures are_equivalent_as_node_list_entails_get_item_pair_are_equivalent_as_node
+      node_list node_list_internal index)
+    (decreases node_list)
+  =
+  if not (are_equivalent_as_node_list_impl node_list node_list_internal) then ()
+  else if not (index < (L.length node_list)) then ()
+  else
+    if index = 0 then
+      assert (are_equivalent_as_node_impl (L.hd node_list) (I.SCons?.hd node_list_internal))
+    else 
+      lemma_are_equivalent_as_node_list_entails_get_item_pair_are_equivalent_as_node
+        (L.tl node_list) (I.SCons?.tl node_list_internal) (index - 1)
+
+let lemma_equivalent_as_node_list_entails_any_item_pair_are_equivalent_as_node (t: eqtype)
+  : Lemma (ensures equivalent_as_node_list_entails_any_item_pair_are_equivalent_as_node t)
+  =
+  introduce forall (node_list_level:nat) (node_list:N.node_list t)
+  (node_list_internal:I.node_list_internal t node_list_level) (index:nat).
+  (are_equivalent_as_node_list_entails_get_item_pair_are_equivalent_as_node
+    node_list node_list_internal index) with
+  (lemma_are_equivalent_as_node_list_entails_get_item_pair_are_equivalent_as_node
+    node_list node_list_internal index)
+
+let lemma_equivalent_as_node_list_entails_both_lengths_are_equal (t: eqtype)
+  : Lemma (ensures equivalent_as_node_list_entails_both_lengths_are_equal t)
   =
   ()
-*)
+  //lemma_to_node_list_theorem t
+
+let lemma_equivalent_theorem (t: eqtype)
+  : Lemma (ensures equivalent_theorem t)
+  =
+  lemma_equivalent_as_node_list_entails_any_item_pair_are_equivalent_as_node t
+
+//---|
+
+//--- theory members ---
+
+let are_equivalent_as_node #t #node_level 
+  (node:N.node t) (node_internal:I.node_internal t node_level)
+  : Pure bool True 
+    (ensures fun _ -> equivalent_theorem t)
+  =
+  lemma_equivalent_theorem t;
+  are_equivalent_as_node_impl node node_internal
+
+let are_equivalent_as_node_list #t #node_list_level
+  (node_list:N.node_list t) (node_list_internal:I.node_list_internal t node_list_level)
+  : Pure bool True
+    (ensures fun _ -> equivalent_theorem t)
+  =
+  lemma_equivalent_theorem t;
+  are_equivalent_as_node_list_impl node_list node_list_internal
 
 //---|
