src/study/Nemonuri.Study.CSharpSyntaxRewriter2.Modifier2/Nemonuri.StratifiedNodes.Nodes.Children.fst
@@ -9,7 +9,10 @@ open Nemonuri.StratifiedNodes.Nodes.Base.Members
 open Nemonuri.StratifiedNodes.Nodes.Bijections
 
 //--- theory members ---
-let get_children #t (node:T.node t) : Tot (T.node_list t) =
+let get_children #t (node:T.node t) 
+  : Pure (T.node_list t) True
+    (ensures fun r -> E.are_equivalent_as_node_list r node.internal.children)
+  =
   to_node_list node.internal.children
 
 let get_children_length #t (node:T.node  t) 
@@ -18,19 +21,27 @@ let get_children_length #t (node:T.node  t)
 //---|
 
 //--- private theory members ---
+
+#push-options "--query_stats"
 let get_child_at #t (node:T.node t) (index:nat)
   : Pure (T.node  t) 
     (requires (index < (get_children_length node)))
-    (ensures fun r -> r = (L.index (get_children node) index))
+    (ensures fun r -> (
+      let node2 = (L.index (get_children node) index) in
+      r = node2)
+    )
   =
+  //assert (E.are_equivalent_as_node_list (get_children node) node.internal.children);
   let node_internal = I.get_item node.internal.children index in (
     //assume ((L.index (get_children node) index).level = (I.get_level node_internal));
     //assume ((L.index (get_children node) index).internal = node_internal);
     assume ( E.are_equivalent_as_node_list_entails_get_item_pair_are_equivalent_as_node
     (get_children node) (node.internal.children) index );
+    //assert (E.are_equivalent_as_node (to_node node_internal) node_internal);
     to_node node_internal
   )
   // TODO: Internals 단계에서 구현하기
   //L.index (get_children nd) index
+#pop-options 
 
 //---|
